\documentclass[12pt]{article}

\usepackage{setspace}
\onehalfspace

\usepackage{amsmath}
\usepackage{moodle}


\begin{document}

\begin{quiz}{valogat}
\begin{multi}{ertek3}
Consider the Hermite interpolational polynomial $H$, for the data:
$$
H(4)=-3 \ \ H(-3)=39 \ \ H'(4)=-20 \ \ H''(4)=-18
$$
Then, $H(1)=$
\item* $ 3 $
\item  $ 6 $
\item  $ 5 $
\item  $ 2 $
\end{multi}\begin{multi}{ertek3}
Consider the Hermite interpolational polynomial $H$, for the data:
$$
H(-4)=114 \ \ H(-2)=26 \ \ H'(-4)=-68 \ \ H''(-4)=28
$$
Then, $H(3)=$
\item* $ -19 $
\item  $ -22 $
\item  $ -23 $
\item  $ -20 $
\end{multi}\begin{multi}{ertek3}
Consider the Hermite interpolational polynomial $H$, for the data:
$$
H(2)=-6 \ \ H(3)=-37 \ \ H'(2)=-18 \ \ H''(2)=-22
$$
Then, $H(4)=$
\item* $ -102 $
\item  $ -99 $
\item  $ -104 $
\item  $ -105 $
\end{multi}\begin{multi}{ertek3}
Consider the Hermite interpolational polynomial $H$, for the data:
$$
H(-3)=-69 \ \ H(-2)=-23 \ \ H'(-3)=67 \ \ H''(-3)=-48
$$
Then, $H(0)=$
\item* $ -3 $
\item  $ 1 $
\item  $ -7 $
\item  $ -1 $
\end{multi}\begin{multi}{ertek3}
Consider the Hermite interpolational polynomial $H$, for the data:
$$
H(0)=-4 \ \ H(-5)=-174 \ \ H'(0)=4 \ \ H''(0)=8
$$
Then, $H(-4)=$
\item* $ -84 $
\item  $ -81 $
\item  $ -80 $
\item  $ -86 $
\end{multi}\begin{multi}{ertek3}
Consider the Hermite interpolational polynomial $H$, for the data:
$$
H(3)=85 \ \ H(1)=3 \ \ H'(3)=85 \ \ H''(3)=56
$$
Then, $H(0)=$
\item* $ 1 $
\item  $ 0 $
\item  $ -2 $
\item  $ -3 $
\end{multi}\begin{multi}{ertek3}
Consider the Hermite interpolational polynomial $H$, for the data:
$$
H(2)=-14 \ \ H(-3)=86 \ \ H'(2)=-30 \ \ H''(2)=-34
$$
Then, $H(0)=$
\item* $ 2 $
\item  $ 5 $
\item  $ 6 $
\item  $ 3 $
\end{multi}\begin{multi}{ertek3}
Consider the Hermite interpolational polynomial $H$, for the data:
$$
H(-3)=-142 \ \ H(4)=236 \ \ H'(-3)=124 \ \ H''(-3)=-76
$$
Then, $H(0)=$
\item* $ -4 $
\item  $ -3 $
\item  $ 0 $
\item  $ -5 $
\end{multi}\begin{multi}{ertek3}
Consider the Hermite interpolational polynomial $H$, for the data:
$$
H(5)=408 \ \ H(3)=88 \ \ H'(5)=242 \ \ H''(5)=94
$$
Then, $H(-3)=$
\item* $ -56 $
\item  $ -52 $
\item  $ -60 $
\item  $ -58 $
\end{multi}\begin{multi}{ertek3}
Consider the Hermite interpolational polynomial $H$, for the data:
$$
H(5)=-408 \ \ H(1)=4 \ \ H'(5)=-267 \ \ H''(5)=-114
$$
Then, $H(3)=$
\item* $ -70 $
\item  $ -74 $
\item  $ -68 $
\item  $ -69 $
\end{multi}\begin{multi}{ertek3}
Consider the Hermite interpolational polynomial $H$, for the data:
$$
H(4)=-256 \ \ H(2)=-42 \ \ H'(4)=-175 \ \ H''(4)=-80
$$
Then, $H(-1)=$
\item* $ -6 $
\item  $ -7 $
\item  $ -3 $
\item  $ -2 $
\end{multi}\begin{multi}{ertek3}
Consider the Hermite interpolational polynomial $H$, for the data:
$$
H(-2)=5 \ \ H(-3)=26 \ \ H'(-2)=-11 \ \ H''(-2)=16
$$
Then, $H(1)=$
\item* $ -10 $
\item  $ -13 $
\item  $ -14 $
\item  $ -6 $
\end{multi}\begin{multi}{ertek3}
Consider the Hermite interpolational polynomial $H$, for the data:
$$
H(2)=-18 \ \ H(4)=-200 \ \ H'(2)=-35 \ \ H''(2)=-40
$$
Then, $H(5)=$
\item* $ -411 $
\item  $ -407 $
\item  $ -412 $
\item  $ -408 $
\end{multi}\begin{multi}{ertek3}
Consider the Hermite interpolational polynomial $H$, for the data:
$$
H(3)=-10 \ \ H(-3)=86 \ \ H'(3)=-28 \ \ H''(3)=-28
$$
Then, $H(-5)=$
\item* $ 342 $
\item  $ 338 $
\item  $ 340 $
\item  $ 343 $
\end{multi}\begin{multi}{ertek3}
Consider the Hermite interpolational polynomial $H$, for the data:
$$
H(3)=-20 \ \ H(-4)=36 \ \ H'(3)=-29 \ \ H''(3)=-20
$$
Then, $H(5)=$
\item* $ -126 $
\item  $ -129 $
\item  $ -127 $
\item  $ -130 $
\end{multi}\begin{multi}{ertek3}
Consider the Hermite interpolational polynomial $H$, for the data:
$$
H(-1)=11 \ \ H(-3)=101 \ \ H'(-1)=-17 \ \ H''(-1)=20
$$
Then, $H(0)=$
\item* $ 2 $
\item  $ -2 $
\item  $ 4 $
\item  $ 5 $
\end{multi}\begin{multi}{ertek3}
Consider the Hermite interpolational polynomial $H$, for the data:
$$
H(-3)=28 \ \ H(-5)=188 \ \ H'(-3)=-40 \ \ H''(-3)=32
$$
Then, $H(3)=$
\item* $ -68 $
\item  $ -65 $
\item  $ -71 $
\item  $ -64 $
\end{multi}\begin{multi}{ertek3}
Consider the Hermite interpolational polynomial $H$, for the data:
$$
H(-5)=289 \ \ H(2)=2 \ \ H'(-5)=-167 \ \ H''(-5)=64
$$
Then, $H(-3)=$
\item* $ 67 $
\item  $ 68 $
\item  $ 71 $
\item  $ 70 $
\end{multi}\begin{multi}{ertek3}
Consider the Hermite interpolational polynomial $H$, for the data:
$$
H(1)=-2 \ \ H(3)=-76 \ \ H'(1)=-9 \ \ H''(1)=-16
$$
Then, $H(-3)=$
\item* $ 98 $
\item  $ 101 $
\item  $ 94 $
\item  $ 95 $
\end{multi}\begin{multi}{ertek3}
Consider the Hermite interpolational polynomial $H$, for the data:
$$
H(-1)=0 \ \ H(-3)=22 \ \ H'(-1)=1 \ \ H''(-1)=4
$$
Then, $H(-2)=$
\item* $ 3 $
\item  $ 5 $
\item  $ 1 $
\item  $ -1 $
\end{multi}\begin{multi}{ertek3}
Consider the Hermite interpolational polynomial $H$, for the data:
$$
H(0)=4 \ \ H(-2)=32 \ \ H'(0)=4 \ \ H''(0)=6
$$
Then, $H(1)=$
\item* $ 8 $
\item  $ 11 $
\item  $ 9 $
\item  $ 7 $
\end{multi}\begin{multi}{ertek3}
Consider the Hermite interpolational polynomial $H$, for the data:
$$
H(-3)=-2 \ \ H(1)=6 \ \ H'(-3)=10 \ \ H''(-3)=-12
$$
Then, $H(-5)=$
\item* $ -54 $
\item  $ -50 $
\item  $ -51 $
\item  $ -57 $
\end{multi}\begin{multi}{ertek3}
Consider the Hermite interpolational polynomial $H$, for the data:
$$
H(0)=-3 \ \ H(4)=-151 \ \ H'(0)=-1 \ \ H''(0)=6
$$
Then, $H(-4)=$
\item* $ 241 $
\item  $ 245 $
\item  $ 244 $
\item  $ 238 $
\end{multi}\begin{multi}{ertek3}
Consider the Hermite interpolational polynomial $H$, for the data:
$$
H(-3)=67 \ \ H(4)=-227 \ \ H'(-3)=-70 \ \ H''(-3)=50
$$
Then, $H(-5)=$
\item* $ 331 $
\item  $ 327 $
\item  $ 332 $
\item  $ 330 $
\end{multi}\begin{multi}{ertek3}
Consider the Hermite interpolational polynomial $H$, for the data:
$$
H(-1)=1 \ \ H(1)=-1 \ \ H'(-1)=-1 \ \ H''(-1)=12
$$
Then, $H(-4)=$
\item* $ 139 $
\item  $ 138 $
\item  $ 140 $
\item  $ 137 $
\end{multi}\begin{multi}{ertek3}
Consider the Hermite interpolational polynomial $H$, for the data:
$$
H(-4)=25 \ \ H(1)=-10 \ \ H'(-4)=-27 \ \ H''(-4)=18
$$
Then, $H(-1)=$
\item* $ -2 $
\item  $ -5 $
\item  $ 0 $
\item  $ 2 $
\end{multi}\begin{multi}{ertek3}
Consider the Hermite interpolational polynomial $H$, for the data:
$$
H(-2)=46 \ \ H(2)=-10 \ \ H'(-2)=-54 \ \ H''(-2)=44
$$
Then, $H(-1)=$
\item* $ 11 $
\item  $ 15 $
\item  $ 10 $
\item  $ 9 $
\end{multi}\begin{multi}{ertek3}
Consider the Hermite interpolational polynomial $H$, for the data:
$$
H(-4)=-211 \ \ H(-3)=-92 \ \ H'(-4)=153 \ \ H''(-4)=-74
$$
Then, $H(2)=$
\item* $ 23 $
\item  $ 27 $
\item  $ 19 $
\item  $ 24 $
\end{multi}\begin{multi}{ertek3}
Consider the Hermite interpolational polynomial $H$, for the data:
$$
H(-3)=-99 \ \ H(-2)=-27 \ \ H'(-3)=103 \ \ H''(-3)=-70
$$
Then, $H(2)=$
\item* $ 41 $
\item  $ 45 $
\item  $ 42 $
\item  $ 39 $
\end{multi}\begin{multi}{ertek3}
Consider the Hermite interpolational polynomial $H$, for the data:
$$
H(2)=19 \ \ H(-1)=-8 \ \ H'(2)=24 \ \ H''(2)=28
$$
Then, $H(-4)=$
\item* $ -269 $
\item  $ -271 $
\item  $ -273 $
\item  $ -270 $
\end{multi}\begin{multi}{ertek3}
Consider the Hermite interpolational polynomial $H$, for the data:
$$
H(-3)=96 \ \ H(3)=-48 \ \ H'(-3)=-96 \ \ H''(-3)=60
$$
Then, $H(0)=$
\item* $ -3 $
\item  $ -5 $
\item  $ -6 $
\item  $ -1 $
\end{multi}\begin{multi}{ertek3}
Consider the Hermite interpolational polynomial $H$, for the data:
$$
H(5)=349 \ \ H(-4)=-92 \ \ H'(5)=184 \ \ H''(5)=66
$$
Then, $H(-3)=$
\item* $ -35 $
\item  $ -36 $
\item  $ -32 $
\item  $ -38 $
\end{multi}\begin{multi}{ertek3}
Consider the Hermite interpolational polynomial $H$, for the data:
$$
H(4)=-158 \ \ H(-3)=59 \ \ H'(4)=-108 \ \ H''(4)=-50
$$
Then, $H(5)=$
\item* $ -293 $
\item  $ -291 $
\item  $ -297 $
\item  $ -296 $
\end{multi}\end{quiz}
\end{document}
