\documentclass[12pt]{article}

\usepackage{setspace}
\onehalfspace

\usepackage{amsmath}
\usepackage{moodle}


\begin{document}

\begin{quiz}{valogat}
\begin{multi}{ertek2}
Let $H$ be the minimal degree polynomial, for which:
$$
H(-5)=253\ \ H(-4)=110 \ \ H'(-5)=-181 \ \ H'(-4)=-108
$$
Then, $H(0)=$
\item* $ -2 $
\item  $ 2 $
\item  $ -1 $
\item  $ 1 $
\end{multi}\begin{multi}{ertek2}
Let $H$ be the minimal degree polynomial, for which:
$$
H(2)=2\ \ H(-5)=-82 \ \ H'(2)=12 \ \ H'(-5)=61
$$
Then, $H(5)=$
\item* $ 128 $
\item  $ 126 $
\item  $ 129 $
\item  $ 124 $
\end{multi}\begin{multi}{ertek2}
Let $H$ be the minimal degree polynomial, for which:
$$
H(-2)=32\ \ H(2)=8 \ \ H'(-2)=-38 \ \ H'(2)=-6
$$
Then, $H(-4)=$
\item* $ 188 $
\item  $ 192 $
\item  $ 187 $
\item  $ 189 $
\end{multi}\begin{multi}{ertek2}
Let $H$ be the minimal degree polynomial, for which:
$$
H(2)=-15\ \ H(-1)=9 \ \ H'(2)=-29 \ \ H'(-1)=-14
$$
Then, $H(-2)=$
\item* $ 37 $
\item  $ 34 $
\item  $ 38 $
\item  $ 36 $
\end{multi}\begin{multi}{ertek2}
Let $H$ be the minimal degree polynomial, for which:
$$
H(5)=181\ \ H(0)=1 \ \ H'(5)=96 \ \ H'(0)=1
$$
Then, $H(-3)=$
\item* $ -11 $
\item  $ -13 $
\item  $ -8 $
\item  $ -12 $
\end{multi}\begin{multi}{ertek2}
Let $H$ be the minimal degree polynomial, for which:
$$
H(0)=3\ \ H(2)=-37 \ \ H'(0)=-2 \ \ H'(2)=-50
$$
Then, $H(-3)=$
\item* $ 63 $
\item  $ 65 $
\item  $ 67 $
\item  $ 61 $
\end{multi}\begin{multi}{ertek2}
Let $H$ be the minimal degree polynomial, for which:
$$
H(4)=-147\ \ H(5)=-283 \ \ H'(4)=-108 \ \ H'(5)=-166
$$
Then, $H(-3)=$
\item* $ 21 $
\item  $ 20 $
\item  $ 24 $
\item  $ 18 $
\end{multi}\begin{multi}{ertek2}
Let $H$ be the minimal degree polynomial, for which:
$$
H(3)=65\ \ H(4)=151 \ \ H'(3)=64 \ \ H'(4)=110
$$
Then, $H(-4)=$
\item* $ -89 $
\item  $ -92 $
\item  $ -85 $
\item  $ -86 $
\end{multi}\begin{multi}{ertek2}
Let $H$ be the minimal degree polynomial, for which:
$$
H(1)=-1\ \ H(5)=307 \ \ H'(1)=5 \ \ H'(5)=197
$$
Then, $H(3)=$
\item* $ 57 $
\item  $ 56 $
\item  $ 54 $
\item  $ 61 $
\end{multi}\begin{multi}{ertek2}
Let $H$ be the minimal degree polynomial, for which:
$$
H(-2)=24\ \ H(-3)=73 \ \ H'(-2)=-30 \ \ H'(-3)=-71
$$
Then, $H(3)=$
\item* $ -101 $
\item  $ -99 $
\item  $ -97 $
\item  $ -98 $
\end{multi}\begin{multi}{ertek2}
Let $H$ be the minimal degree polynomial, for which:
$$
H(0)=-2\ \ H(-5)=578 \ \ H'(0)=4 \ \ H'(-5)=-336
$$
Then, $H(-2)=$
\item* $ 38 $
\item  $ 34 $
\item  $ 41 $
\item  $ 36 $
\end{multi}\begin{multi}{ertek2}
Let $H$ be the minimal degree polynomial, for which:
$$
H(-2)=-40\ \ H(0)=-4 \ \ H'(-2)=46 \ \ H'(0)=2
$$
Then, $H(4)=$
\item* $ 164 $
\item  $ 165 $
\item  $ 168 $
\item  $ 163 $
\end{multi}\begin{multi}{ertek2}
Let $H$ be the minimal degree polynomial, for which:
$$
H(-3)=79\ \ H(5)=-329 \ \ H'(-3)=-83 \ \ H'(5)=-211
$$
Then, $H(0)=$
\item* $ 1 $
\item  $ -2 $
\item  $ -3 $
\item  $ 4 $
\end{multi}\begin{multi}{ertek2}
Let $H$ be the minimal degree polynomial, for which:
$$
H(-2)=14\ \ H(2)=10 \ \ H'(-2)=-17 \ \ H'(2)=-1
$$
Then, $H(-5)=$
\item* $ 164 $
\item  $ 168 $
\item  $ 167 $
\item  $ 163 $
\end{multi}\begin{multi}{ertek2}
Let $H$ be the minimal degree polynomial, for which:
$$
H(2)=-7\ \ H(0)=-3 \ \ H'(2)=6 \ \ H'(0)=-2
$$
Then, $H(-5)=$
\item* $ -343 $
\item  $ -347 $
\item  $ -340 $
\item  $ -346 $
\end{multi}\begin{multi}{ertek2}
Let $H$ be the minimal degree polynomial, for which:
$$
H(-2)=-12\ \ H(-4)=-108 \ \ H'(-2)=18 \ \ H'(-4)=86
$$
Then, $H(-5)=$
\item* $ -219 $
\item  $ -216 $
\item  $ -217 $
\item  $ -222 $
\end{multi}\begin{multi}{ertek2}
Let $H$ be the minimal degree polynomial, for which:
$$
H(0)=-2\ \ H(-5)=-442 \ \ H'(0)=-2 \ \ H'(-5)=253
$$
Then, $H(-3)=$
\item* $ -104 $
\item  $ -102 $
\item  $ -106 $
\item  $ -107 $
\end{multi}\begin{multi}{ertek2}
Let $H$ be the minimal degree polynomial, for which:
$$
H(4)=86\ \ H(-5)=-112 \ \ H'(4)=58 \ \ H'(-5)=67
$$
Then, $H(-1)=$
\item* $ -4 $
\item  $ -8 $
\item  $ -6 $
\item  $ -7 $
\end{multi}\begin{multi}{ertek2}
Let $H$ be the minimal degree polynomial, for which:
$$
H(-5)=341\ \ H(-3)=73 \ \ H'(-5)=-208 \ \ H'(-3)=-72
$$
Then, $H(0)=$
\item* $ 1 $
\item  $ -2 $
\item  $ -1 $
\item  $ 0 $
\end{multi}\begin{multi}{ertek2}
Let $H$ be the minimal degree polynomial, for which:
$$
H(3)=-114\ \ H(-3)=54 \ \ H'(3)=-100 \ \ H'(-3)=-64
$$
Then, $H(-4)=$
\item* $ 145 $
\item  $ 141 $
\item  $ 143 $
\item  $ 146 $
\end{multi}\begin{multi}{ertek2}
Let $H$ be the minimal degree polynomial, for which:
$$
H(-3)=-94\ \ H(5)=154 \ \ H'(-3)=79 \ \ H'(5)=111
$$
Then, $H(0)=$
\item* $ -1 $
\item  $ -4 $
\item  $ -2 $
\item  $ 0 $
\end{multi}\begin{multi}{ertek2}
Let $H$ be the minimal degree polynomial, for which:
$$
H(3)=45\ \ H(5)=287 \ \ H'(3)=61 \ \ H'(5)=193
$$
Then, $H(-5)=$
\item* $ -443 $
\item  $ -442 $
\item  $ -446 $
\item  $ -444 $
\end{multi}\begin{multi}{ertek2}
Let $H$ be the minimal degree polynomial, for which:
$$
H(-1)=-1\ \ H(-5)=259 \ \ H'(-1)=3 \ \ H'(-5)=-181
$$
Then, $H(5)=$
\item* $ -451 $
\item  $ -447 $
\item  $ -455 $
\item  $ -452 $
\end{multi}\begin{multi}{ertek2}
Let $H$ be the minimal degree polynomial, for which:
$$
H(3)=24\ \ H(-3)=-12 \ \ H'(3)=30 \ \ H'(-3)=18
$$
Then, $H(-5)=$
\item* $ -88 $
\item  $ -91 $
\item  $ -89 $
\item  $ -90 $
\end{multi}\begin{multi}{ertek2}
Let $H$ be the minimal degree polynomial, for which:
$$
H(-3)=87\ \ H(4)=-263 \ \ H'(-3)=-99 \ \ H'(4)=-197
$$
Then, $H(1)=$
\item* $ -5 $
\item  $ -3 $
\item  $ -9 $
\item  $ -7 $
\end{multi}\begin{multi}{ertek2}
Let $H$ be the minimal degree polynomial, for which:
$$
H(1)=2\ \ H(0)=-1 \ \ H'(1)=3 \ \ H'(0)=2
$$
Then, $H(-3)=$
\item* $ 38 $
\item  $ 42 $
\item  $ 39 $
\item  $ 41 $
\end{multi}\begin{multi}{ertek2}
Let $H$ be the minimal degree polynomial, for which:
$$
H(-2)=50\ \ H(0)=4 \ \ H'(-2)=-61 \ \ H'(0)=-1
$$
Then, $H(-3)=$
\item* $ 142 $
\item  $ 140 $
\item  $ 144 $
\item  $ 139 $
\end{multi}\begin{multi}{ertek2}
Let $H$ be the minimal degree polynomial, for which:
$$
H(2)=12\ \ H(0)=-4 \ \ H'(2)=20 \ \ H'(0)=4
$$
Then, $H(-4)=$
\item* $ -180 $
\item  $ -176 $
\item  $ -177 $
\item  $ -179 $
\end{multi}\begin{multi}{ertek2}
Let $H$ be the minimal degree polynomial, for which:
$$
H(-1)=6\ \ H(-5)=-34 \ \ H'(-1)=-6 \ \ H'(-5)=42
$$
Then, $H(-4)=$
\item* $ -3 $
\item  $ 1 $
\item  $ -6 $
\item  $ -5 $
\end{multi}\begin{multi}{ertek2}
Let $H$ be the minimal degree polynomial, for which:
$$
H(-3)=-73\ \ H(-4)=-141 \ \ H'(-3)=54 \ \ H'(-4)=83
$$
Then, $H(-2)=$
\item* $ -31 $
\item  $ -35 $
\item  $ -27 $
\item  $ -29 $
\end{multi}\begin{multi}{ertek2}
Let $H$ be the minimal degree polynomial, for which:
$$
H(5)=144\ \ H(3)=32 \ \ H'(5)=84 \ \ H'(3)=32
$$
Then, $H(4)=$
\item* $ 75 $
\item  $ 77 $
\item  $ 74 $
\item  $ 72 $
\end{multi}\begin{multi}{ertek2}
Let $H$ be the minimal degree polynomial, for which:
$$
H(5)=-342\ \ H(-1)=-6 \ \ H'(5)=-188 \ \ H'(-1)=4
$$
Then, $H(1)=$
\item* $ -6 $
\item  $ -10 $
\item  $ -7 $
\item  $ -2 $
\end{multi}\begin{multi}{ertek2}
Let $H$ be the minimal degree polynomial, for which:
$$
H(5)=-208\ \ H(0)=-3 \ \ H'(5)=-131 \ \ H'(0)=-1
$$
Then, $H(-4)=$
\item* $ 161 $
\item  $ 165 $
\item  $ 158 $
\item  $ 163 $
\end{multi}\end{quiz}
\end{document}
