\documentclass[12pt]{article}

\usepackage{setspace}
\onehalfspace

\usepackage{amsmath}
\usepackage{moodle}


\begin{document}

\begin{quiz}{valogat}
\begin{multi}{ertek}
If $H$ is the minimal degree polynomial, for which:
$$
H(2)=8 \ \  H(-1)=-7 \ \ H'(2)=8
$$
Then, $H(-3)=$
\item* $ -7 $
\item  $ -10 $
\item  $ -8 $
\item  $ -4 $
\end{multi}
\begin{multi}{ertek}
If $H$ is the minimal degree polynomial, for which:
$$
H(-3)=22 \ \  H(3)=46 \ \ H'(-3)=-20
$$
Then, $H(0)=$
\item* $ -2 $
\item  $ 0 $
\item  $ -1 $
\item  $ -4 $
\end{multi}
\begin{multi}{ertek}
If $H$ is the minimal degree polynomial, for which:
$$
H(-1)=-6 \ \  H(2)=-21 \ \ H'(-1)=7
$$
Then, $H(3)=$
\item* $ -42 $
\item  $ -45 $
\item  $ -39 $
\item  $ -38 $
\end{multi}
\begin{multi}{ertek}
If $H$ is the minimal degree polynomial, for which:
$$
H(4)=21 \ \  H(-4)=13 \ \ H'(4)=9
$$
Then, $H(-3)=$
\item* $ 7 $
\item  $ 4 $
\item  $ 3 $
\item  $ 8 $
\end{multi}
\begin{multi}{ertek}
If $H$ is the minimal degree polynomial, for which:
$$
H(-3)=-17 \ \  H(-1)=3 \ \ H'(-3)=16
$$
Then, $H(2)=$
\item* $ -12 $
\item  $ -9 $
\item  $ -8 $
\item  $ -13 $
\end{multi}
\begin{multi}{ertek}
If $H$ is the minimal degree polynomial, for which:
$$
H(4)=-84 \ \  H(2)=-28 \ \ H'(4)=-36
$$
Then, $H(3)=$
\item* $ -52 $
\item  $ -51 $
\item  $ -54 $
\item  $ -55 $
\end{multi}
\begin{multi}{ertek}
If $H$ is the minimal degree polynomial, for which:
$$
H(-4)=-72 \ \  H(-3)=-41 \ \ H'(-4)=35
$$
Then, $H(3)=$
\item* $ -23 $
\item  $ -27 $
\item  $ -25 $
\item  $ -20 $
\end{multi}
\begin{multi}{ertek}
If $H$ is the minimal degree polynomial, for which:
$$
H(-2)=2 \ \  H(0)=-4 \ \ H'(-2)=-9
$$
Then, $H(3)=$
\item* $ 32 $
\item  $ 36 $
\item  $ 34 $
\item  $ 33 $
\end{multi}
\begin{multi}{ertek}
If $H$ is the minimal degree polynomial, for which:
$$
H(1)=-1 \ \  H(-3)=-29 \ \ H'(1)=-1
$$
Then, $H(-1)=$
\item* $ -7 $
\item  $ -10 $
\item  $ -4 $
\item  $ -9 $
\end{multi}
\begin{multi}{ertek}
If $H$ is the minimal degree polynomial, for which:
$$
H(-2)=-15 \ \  H(-3)=-34 \ \ H'(-2)=15
$$
Then, $H(1)=$
\item* $ -6 $
\item  $ -7 $
\item  $ -4 $
\item  $ -3 $
\end{multi}
\begin{multi}{ertek}
If $H$ is the minimal degree polynomial, for which:
$$
H(4)=26 \ \  H(-2)=-4 \ \ H'(4)=11
$$
Then, $H(3)=$
\item* $ 16 $
\item  $ 17 $
\item  $ 15 $
\item  $ 12 $
\end{multi}
\begin{multi}{ertek}
If $H$ is the minimal degree polynomial, for which:
$$
H(-1)=-4 \ \  H(-3)=-36 \ \ H'(-1)=10
$$
Then, $H(-2)=$
\item* $ -17 $
\item  $ -14 $
\item  $ -15 $
\item  $ -19 $
\end{multi}
\begin{multi}{ertek}
If $H$ is the minimal degree polynomial, for which:
$$
H(-1)=9 \ \  H(3)=9 \ \ H'(-1)=-8
$$
Then, $H(1)=$
\item* $ 1 $
\item  $ -2 $
\item  $ 4 $
\item  $ 0 $
\end{multi}
\begin{multi}{ertek}
If $H$ is the minimal degree polynomial, for which:
$$
H(-2)=14 \ \  H(0)=2 \ \ H'(-2)=-14
$$
Then, $H(3)=$
\item* $ 44 $
\item  $ 41 $
\item  $ 46 $
\item  $ 45 $
\end{multi}
\begin{multi}{ertek}
If $H$ is the minimal degree polynomial, for which:
$$
H(-3)=-43 \ \  H(-2)=-20 \ \ H'(-3)=27
$$
Then, $H(4)=$
\item* $ -50 $
\item  $ -51 $
\item  $ -47 $
\item  $ -48 $
\end{multi}
\begin{multi}{ertek}
If $H$ is the minimal degree polynomial, for which:
$$
H(4)=31 \ \  H(-1)=1 \ \ H'(4)=11
$$
Then, $H(-2)=$
\item* $ 1 $
\item  $ -2 $
\item  $ 4 $
\item  $ 5 $
\end{multi}
\begin{multi}{ertek}
If $H$ is the minimal degree polynomial, for which:
$$
H(-2)=0 \ \  H(3)=-20 \ \ H'(-2)=6
$$
Then, $H(0)=$
\item* $ 4 $
\item  $ 6 $
\item  $ 8 $
\item  $ 0 $
\end{multi}
\begin{multi}{ertek}
If $H$ is the minimal degree polynomial, for which:
$$
H(4)=-41 \ \  H(2)=-9 \ \ H'(4)=-22
$$
Then, $H(-2)=$
\item* $ -17 $
\item  $ -20 $
\item  $ -19 $
\item  $ -15 $
\end{multi}
\begin{multi}{ertek}
If $H$ is the minimal degree polynomial, for which:
$$
H(4)=-67 \ \  H(-2)=-13 \ \ H'(4)=-33
$$
Then, $H(3)=$
\item* $ -38 $
\item  $ -41 $
\item  $ -36 $
\item  $ -35 $
\end{multi}
\begin{multi}{ertek}
If $H$ is the minimal degree polynomial, for which:
$$
H(1)=0 \ \  H(3)=0 \ \ H'(1)=-2
$$
Then, $H(-2)=$
\item* $ 15 $
\item  $ 11 $
\item  $ 19 $
\item  $ 18 $
\end{multi}
\begin{multi}{ertek}
If $H$ is the minimal degree polynomial, for which:
$$
H(1)=-3 \ \  H(0)=1 \ \ H'(1)=-7
$$
Then, $H(-4)=$
\item* $ -43 $
\item  $ -42 $
\item  $ -44 $
\item  $ -46 $
\end{multi}
\begin{multi}{ertek}
If $H$ is the minimal degree polynomial, for which:
$$
H(-3)=-22 \ \  H(-4)=-33 \ \ H'(-3)=10
$$
Then, $H(-1)=$
\item* $ -6 $
\item  $ -7 $
\item  $ -5 $
\item  $ -9 $
\end{multi}
\begin{multi}{ertek}
If $H$ is the minimal degree polynomial, for which:
$$
H(0)=4 \ \  H(1)=2 \ \ H'(0)=-1
$$
Then, $H(3)=$
\item* $ -8 $
\item  $ -5 $
\item  $ -4 $
\item  $ -12 $
\end{multi}
\begin{multi}{ertek}
If $H$ is the minimal degree polynomial, for which:
$$
H(-1)=2 \ \  H(0)=-3 \ \ H'(-1)=-8
$$
Then, $H(2)=$
\item* $ 5 $
\item  $ 3 $
\item  $ 1 $
\item  $ 6 $
\end{multi}
\begin{multi}{ertek}
If $H$ is the minimal degree polynomial, for which:
$$
H(2)=-3 \ \  H(-4)=-57 \ \ H'(2)=-9
$$
Then, $H(-3)=$
\item* $ -33 $
\item  $ -30 $
\item  $ -36 $
\item  $ -29 $
\end{multi}
\begin{multi}{ertek}
If $H$ is the minimal degree polynomial, for which:
$$
H(-4)=28 \ \  H(-2)=8 \ \ H'(-4)=-14
$$
Then, $H(3)=$
\item* $ 28 $
\item  $ 24 $
\item  $ 32 $
\item  $ 27 $
\end{multi}
\begin{multi}{ertek}
If $H$ is the minimal degree polynomial, for which:
$$
H(-2)=18 \ \  H(1)=0 \ \ H'(-2)=-12
$$
Then, $H(3)=$
\item* $ 8 $
\item  $ 11 $
\item  $ 5 $
\item  $ 9 $
\end{multi}
\begin{multi}{ertek}
If $H$ is the minimal degree polynomial, for which:
$$
H(-2)=5 \ \  H(2)=21 \ \ H'(-2)=-8
$$
Then, $H(-1)=$
\item* $ 0 $
\item  $ 4 $
\item  $ -2 $
\item  $ -4 $
\end{multi}
\begin{multi}{ertek}
If $H$ is the minimal degree polynomial, for which:
$$
H(-1)=-6 \ \  H(3)=-6 \ \ H'(-1)=4
$$
Then, $H(2)=$
\item* $ -3 $
\item  $ -5 $
\item  $ -6 $
\item  $ 0 $
\end{multi}
\begin{multi}{ertek}
If $H$ is the minimal degree polynomial, for which:
$$
H(-1)=5 \ \  H(-2)=11 \ \ H'(-1)=-5
$$
Then, $H(1)=$
\item* $ -1 $
\item  $ 3 $
\item  $ -4 $
\item  $ 2 $
\end{multi}
\begin{multi}{ertek}
If $H$ is the minimal degree polynomial, for which:
$$
H(2)=22 \ \  H(-2)=14 \ \ H'(2)=18
$$
Then, $H(-1)=$
\item* $ 4 $
\item  $ 8 $
\item  $ 7 $
\item  $ 3 $
\end{multi}
\begin{multi}{ertek}
If $H$ is the minimal degree polynomial, for which:
$$
H(-4)=2 \ \  H(-1)=-4 \ \ H'(-4)=-5
$$
Then, $H(3)=$
\item* $ 16 $
\item  $ 20 $
\item  $ 13 $
\item  $ 18 $
\end{multi}
\begin{multi}{ertek}
If $H$ is the minimal degree polynomial, for which:
$$
H(-3)=14 \ \  H(0)=-1 \ \ H'(-3)=-11
$$
Then, $H(-4)=$
\item* $ 27 $
\item  $ 24 $
\item  $ 31 $
\item  $ 25 $
\end{multi}
\end{quiz}
\end{document}
